verif/HMAC_verif.v
@@ -34,11 +34,13 @@ Ltac ec := econstructor; try unfold mb; try reflexivity.
 Ltac fg := eapply eager_eval_global_var; [ reflexivity | eassumption | idtac].
 Ltac g := eapply eager_eval_global_var; try eassumption; try reflexivity.
 
+
 Ltac e :=
   match goal with
-  | [ |- eager_eval_expr _ ?E (EVar ?id) _ ] =>
-    try fg; try reflexivity;
-    try solve [eapply eager_eval_local_var; reflexivity]
+  | [ |- eager_eval_expr ?GE _ ?E (EVar ?id) _ ] =>
+    (try fg); (try reflexivity);
+    (try solve [eapply eager_eval_local_var; reflexivity]);
+    fail 1 "couldn't figure out variable"
   | [ |- _ ] => ec
   end.
 
@@ -52,8 +54,10 @@ Lemma kinit_eval :
   forall k,
     n_bits 64 k ->
     forall h,
+      (exists hv,
+          eager_eval_expr ge tempty sempty h hv) ->
     exists v,
-      eager_eval_expr ge tempty sempty (apply (tapply (EVar kinit) (pwBytes :: blockLength :: digest ::  nil)) (h :: (EList (map EValue k)) :: nil)) v.
+      eager_eval_expr ge tempty sempty (apply (tapply (EVar kinit) (pwBytes :: blockLength :: digest ::  nil)) (h :: (EList (map EValue k)) :: nil)) v /\ eager_eval_expr ge tempty sempty (EList (map EValue k)) v.
 Proof.
   init_globals ge.
   intros.
@@ -62,60 +66,60 @@ Proof.
   destruct H. instantiate (3 := ge) in H.
   instantiate (1 := sempty) in H.
   instantiate (1 := tempty) in H.
+  destruct H.
+  inversion H. subst.
+  destruct H0.
+  eexists. split; try eassumption. unfold apply.
   
-  
-  eexists. unfold apply.
   e. e.
-  e. e. e. g. e. repeat e.
+  e. e. e.
+  
+  g.
+  e. e. repeat e.
   e. repeat e.
   e. repeat e.
-  e.
-  admit. (* hash evaluates to some closure *)
+  eassumption.
   e. 
   eassumption.
   e. e. e. e. g. e. repeat e.
   e. e. e. g. e.
   repeat e. repeat e.
   simpl. repeat e.
-  simpl. e. repe
+  simpl. e. repeat e.
   repeat e. repeat e. 
   
 
   
-  e. e. e. e. e. repeat e.
-  e. repeat e. e. repeat e. simpl. reflexivity.
-  e. repeat e.
-  simpl. reflexivity.
-  simpl. e.
-  e. e. e.
+  e. e. e. fg. repeat e.
+  e. repeat e. e. repeat e. repeat e.
+  repeat e. repeat e.
+  simpl.
 
-  g. e. repeat e.
+  e. e. e. e. g.
+  repeat e. repeat e.
   e. repeat e.
-  e. repeat e. e. e. e. repeat e.
-  e. e. e. g. e. repeat e. repeat e.
   e. repeat e.
+  e. e. e. e. e. e. g.
+  repeat e. e. e. repeat e.
+  e. repeat e. e. e. e. e. g.
+  repeat e. repeat e.
+  repeat e. repeat e.
 
-  rewrite append_strict_list. reflexivity.
+  rewrite append_strict_list. reflexivity.  
   
-  e.
-  eapply eager_eval_global_var. simpl. reflexivity.
-  simpl. reflexivity.
-  e. eapply eager_eval_global_var. simpl. reflexivity.
-  simpl. reflexivity.
+  e. g. e. g.
+  e. e. e. e. g.
+  all: try solve [repeat e].
+  e. repeat e. repeat e.
 
 
-  e. e. e. e. g. e.
+  replace (tnum 64) with (tnum (Z.of_nat (Datatypes.length x))).
+  rewrite splitAt_len. reflexivity.
   
-  admit. (* type variable numbering *)
-  e. admit. (* type variable numbering *)
-  e. admit. (* type variable numbering *)
+  f_equal. omega.
+  simpl. reflexivity.
 
-  e. eapply eager_eval_local_var. reflexivity.
-  e. repeat e.
-
-  (* Now need a minor lemma about split_at giving back same thing, but that should be easy once we fix type variable numbering *)
-  
-Admitted.
+Qed.
 
 
 
