verif/SplitB.v
@@ -22,7 +22,7 @@ Require Import Split.
 
 Lemma eval_b :
   exists v,
-    eval_expr ge empty (EVar b) v /\ force_list ge empty v (@from_bitv 8 (@repr 8 2)).
+    eval_expr ge tempty empty (EVar b) v /\ force_list ge tempty empty v (@from_bitv 8 (@repr 8 2)).
 Proof.
   init_globals ge.
   eexists; split.
